LF-Church: termination and reducibility in Type

src/LF-Church/termination_LF.hs
@@ -1,0 +1,278 @@
+{-# OPTIONS_GHC -cpp -fglasgow-exts #-}
+{- For Hugs, use the option -F"cpp -P -traditional" -}
+
+module Termination_LF where
+
+import qualified Prelude
+
+
+unsafeCoerce :: a -> b
+#ifdef __GLASGOW_HASKELL__
+import qualified GHC.Base
+unsafeCoerce = GHC.Base.unsafeCoerce#
+#else
+-- HUGS
+import qualified IOExts
+unsafeCoerce = IOExts.unsafeCoerce
+#endif
+
+__ :: any
+__ = Prelude.error "Logical or arity value used"
+
+false_rect :: a1
+false_rect =
+  Prelude.error "absurd case"
+
+eq_rect :: a1 -> a2 -> a1 -> a2
+eq_rect x f y =
+  f
+
+data Option a =
+   Some a
+ | None
+
+type Sig a =
+  a
+  -- singleton inductive, whose constructor was exist
+  
+proj1_sig :: a1 -> a1
+proj1_sig e =
+  e
+
+plus :: int -> int -> int
+plus = ( + )
+
+indefinite_description :: a1
+indefinite_description =
+  Prelude.error "AXIOM TO BE REALIZED"
+
+classicT :: bool
+classicT =
+  case indefinite_description of {
+   true -> true;
+   false -> false}
+
+type Decidable =
+  bool
+  -- singleton inductive, whose constructor was decidable_make
+  
+type Comparable a =
+  a -> a -> Decidable
+  -- singleton inductive, whose constructor was make_comparable
+  
+nat_compare :: int -> int -> bool
+nat_compare x y =
+  (fun zero succ n →       if n=0 then zero () else succ (n-1))
+    (\_ ->
+    (fun zero succ n →       if n=0 then zero () else succ (n-1))
+      (\_ ->
+      true)
+      (\n ->
+      false)
+      y)
+    (\x' ->
+    (fun zero succ n →       if n=0 then zero () else succ (n-1))
+      (\_ ->
+      false)
+      (\y' ->
+      nat_compare x' y')
+      y)
+    x
+
+nat_comparable :: Comparable int
+nat_comparable x y =
+  nat_compare x y
+
+inhab_witness :: a1
+inhab_witness =
+  indefinite_description
+
+epsilon_def :: a1
+epsilon_def =
+  case classicT of {
+   true -> indefinite_description;
+   false -> inhab_witness}
+
+epsilon :: a1
+epsilon =
+  proj1_sig epsilon_def
+
+fold_right :: (a1 -> a2 -> a2) -> a2 -> (list a1) -> a2
+fold_right f acc l =
+  case l of {
+   [] -> acc;
+   (::) x l' -> f x (fold_right f acc l')}
+
+type Set a = ()
+
+type Fset a = (Set a)
+
+build_fset :: (Set a1)
+build_fset =
+  __
+
+empty :: Fset a1
+empty =
+  build_fset
+
+singleton :: a1 -> (Set a1)
+singleton x =
+  build_fset
+
+union :: (Fset a1) -> (Fset a1) -> (Set a1)
+union e f =
+  build_fset
+
+inter :: (Fset a1) -> (Fset a1) -> (Set a1)
+inter e f =
+  build_fset
+
+remove :: (Fset a1) -> (Fset a1) -> (Set a1)
+remove e f =
+  build_fset
+
+from_list :: (list a1) -> Fset a1
+from_list l =
+  fold_right (\x acc -> union (singleton x) acc) empty l
+
+type Var = int
+
+var_comp :: Comparable Var
+var_comp =
+  nat_comparable
+
+var_comparable :: Comparable Var
+var_comparable =
+  var_comp
+
+type Vars = Fset Var
+
+var_gen_list :: (list int) -> int
+var_gen_list l =
+  plus ((fun x → x + 1) 0) (fold_right plus 0 l)
+
+var_gen :: Vars -> Var
+var_gen e =
+  var_gen_list epsilon
+
+var_fresh :: Vars -> Var
+var_fresh l =
+  var_gen l
+
+data Ty =
+   Tvar
+ | Tarrow Ty Ty
+ | Tbox Ty
+ | Tdia Ty
+
+ty_rect :: a1 -> (Ty -> a1 -> Ty -> a1 -> a1) -> (Ty -> a1 -> a1) -> (Ty ->
+           a1 -> a1) -> Ty -> a1
+ty_rect f f0 f1 f2 t =
+  case t of {
+   Tvar -> f;
+   Tarrow t0 t1 -> f0 t0 (ty_rect f f0 f1 f2 t0) t1 (ty_rect f f0 f1 f2 t1);
+   Tbox t0 -> f1 t0 (ty_rect f f0 f1 f2 t0);
+   Tdia t0 -> f2 t0 (ty_rect f f0 f1 f2 t0)}
+
+data Vte =
+   Bte int
+ | Fte Var
+
+eq_var_dec :: Var -> Var -> bool
+eq_var_dec = ( = )
+
+type Ctx_LF = list ((*) Var Ty)
+
+type Bg_LF = list Ctx_LF
+
+data Te_LF =
+   Hyp_LF Vte
+ | Lam_LF Ty Te_LF
+ | Appl_LF Te_LF Te_LF
+ | Box_LF Te_LF
+ | Unbox_LF Te_LF
+ | Here_LF Te_LF
+ | Letdia_LF Ty Te_LF Te_LF
+
+emptyEquiv_LF :: (list (list ((*) Var Ty))) -> list (list ((*) Var Ty))
+emptyEquiv_LF g =
+  case g of {
+   [] -> [];
+   (::) a g' -> (::) [] (emptyEquiv_LF g')}
+
+find_var :: (list ((*) ((*) Var Ty) Te_LF)) -> Var -> Option
+            ((*) ((*) Var Ty) Te_LF)
+find_var l x =
+  case l of {
+   [] -> None;
+   (::) p l' ->
+    case p of {
+     (,) p0 m ->
+      case p0 of {
+       (,) v a ->
+        case eq_var_dec x v of {
+         true -> Some ((,) ((,) v a) m);
+         false -> find_var l' x}}}}
+
+sL :: (list ((*) ((*) Var Ty) Te_LF)) -> Te_LF -> Te_LF
+sL l m =
+  case m of {
+   Hyp_LF v0 ->
+    case v0 of {
+     Bte v -> m;
+     Fte v ->
+      let {x = find_var l v} in
+      case x of {
+       Some p ->
+        case p of {
+         (,) p0 m0 -> m0};
+       None -> Hyp_LF (Fte v)}};
+   Lam_LF a m0 -> Lam_LF a (sL l m0);
+   Appl_LF m0 n -> Appl_LF (sL l m0) (sL l n);
+   Box_LF m0 -> Box_LF (sL l m0);
+   Unbox_LF m0 -> Unbox_LF (sL l m0);
+   Here_LF m0 -> Here_LF (sL l m0);
+   Letdia_LF t m0 n -> Letdia_LF t (sL l m0) (sL l n)}
+
+type WT = Te_LF
+
+wT_here :: Te_LF -> WT -> WT
+wT_here m x =
+  Here_LF x
+
+data Cont =
+   IdK Ty
+ | ConsU Cont Ty
+ | ConsD Cont Ty Te_LF Ty Ty
+ | ConsA Cont Te_LF Ty Ty
+
+type RC = ()
+
+type Q = Cont -> () -> () -> RC -> WT
+
+rCIdK :: Ty -> RC
+rCIdK t =
+  ty_rect (unsafeCoerce (\v _ x -> x)) (\t1 iHt1 t2 iHt2 ->
+    unsafeCoerce (\v _ x ->
+      case x of {
+       (,) w w0 -> w})) (\t0 iHt ->
+    unsafeCoerce (\v _ x ->
+      case x of {
+       (,) w w0 -> w})) (\t0 iHt ->
+    unsafeCoerce (\v _ x -> let {x0 = x (IdK t0) __ __ iHt} in wT_here v x0))
+    t
+
+main_theorem :: Bg_LF -> Ctx_LF -> Te_LF -> Ty -> (list
+                ((*) ((*) Var Ty) Te_LF)) -> (Var -> Ty -> Te_LF -> () -> Q)
+                -> Cont -> RC -> WT
+main_theorem =
+  Prelude.error "AXIOM TO BE REALIZED"
+
+wT_Lang :: (list (list ((*) Var Ty))) -> Te_LF -> Ty -> WT
+wT_Lang g m a =
+  let {
+   h = main_theorem (emptyEquiv_LF g) [] m a [] (\a0 b c _ -> false_rect)
+         (IdK a) (rCIdK a)}
+  in
+  eq_rect (sL [] m) h m
+
